Base Dead Code Elim on Subst01
Based on https://github.com/coq/coq/issues/8993#issuecomment-438572277,
I am guessing that DCE is currently memory-hungry.  This makes sense,
because every [var] is carrying around a full `PositiveSet.t` when
computing live variables.  Instead, we now adjust `subst01` to not
increment counts coming from dead variables, and use it to implement
DCE.  Hopefully this will be much faster and more efficient.

After     | File Name                                                            | Before    || Change     | % Change
---------------------------------------------------------------------------------------------------------------------
40m52.19s | Total                                                                | 26m17.07s || +14m35.12s | +55.49%
---------------------------------------------------------------------------------------------------------------------
21m50.67s | p384_32.c                                                            | 7m10.69s  || +14m39.98s | +204.31%
4m44.43s  | Experiments/NewPipeline/Toplevel1.vo                                 | 4m57.77s  || -0m13.33s  | -4.47%
0m32.80s  | secp256k1_32.c                                                       | 0m19.76s  || +0m13.03s  | +65.99%
0m32.31s  | p256_32.c                                                            | 0m18.82s  || +0m13.49s  | +71.67%
6m22.37s  | Experiments/NewPipeline/SlowPrimeSynthesisExamples.vo                | 6m33.72s  || -0m11.35s  | -2.88%
0m11.63s  | p224_32.c                                                            | 0m08.43s  || +0m03.20s  | +37.95%
1m33.11s  | Experiments/NewPipeline/Toplevel2.vo                                 | 1m35.89s  || -0m02.78s  | -2.89%
0m41.93s  | Experiments/NewPipeline/ExtractionOCaml/word_by_word_montgomery      | 0m43.28s  || -0m01.35s  | -3.11%
0m40.89s  | Experiments/NewPipeline/ExtractionHaskell/word_by_word_montgomery    | 0m41.99s  || -0m01.10s  | -2.61%
0m18.65s  | Experiments/NewPipeline/ExtractionHaskell/saturated_solinas          | 0m19.77s  || -0m01.12s  | -5.66%
0m02.65s  | Experiments/NewPipeline/MiscCompilerPassesProofs.vo                  | 0m03.86s  || -0m01.20s  | -31.34%
0m40.46s  | p521_32.c                                                            | 0m40.32s  || +0m00.14s  | +0.34%
0m33.94s  | p521_64.c                                                            | 0m33.47s  || +0m00.46s  | +1.40%
0m25.60s  | Experiments/NewPipeline/ExtractionHaskell/unsaturated_solinas        | 0m26.33s  || -0m00.72s  | -2.77%
0m23.85s  | Experiments/NewPipeline/ExtractionOCaml/unsaturated_solinas          | 0m24.62s  || -0m00.76s  | -3.12%
0m15.77s  | Experiments/NewPipeline/ExtractionOCaml/saturated_solinas            | 0m16.23s  || -0m00.46s  | -2.83%
0m11.70s  | p384_64.c                                                            | 0m11.61s  || +0m00.08s  | +0.77%
0m09.18s  | Experiments/NewPipeline/ExtractionOCaml/word_by_word_montgomery.ml   | 0m09.46s  || -0m00.28s  | -2.95%
0m06.00s  | Experiments/NewPipeline/ExtractionHaskell/word_by_word_montgomery.hs | 0m06.04s  || -0m00.04s  | -0.66%
0m05.94s  | Experiments/NewPipeline/ExtractionOCaml/unsaturated_solinas.ml       | 0m06.20s  || -0m00.25s  | -4.19%
0m04.47s  | Experiments/NewPipeline/ExtractionHaskell/unsaturated_solinas.hs     | 0m04.52s  || -0m00.04s  | -1.10%
0m04.40s  | Experiments/NewPipeline/ExtractionOCaml/saturated_solinas.ml         | 0m04.72s  || -0m00.31s  | -6.77%
0m03.76s  | Experiments/NewPipeline/ExtractionHaskell/saturated_solinas.hs       | 0m03.78s  || -0m00.02s  | -0.52%
0m02.36s  | curve25519_32.c                                                      | 0m02.31s  || +0m00.04s  | +2.16%
0m02.10s  | secp256k1_64.c                                                       | 0m02.14s  || -0m00.04s  | -1.86%
0m02.05s  | p256_64.c                                                            | 0m02.07s  || -0m00.02s  | -0.96%
0m01.94s  | p224_64.c                                                            | 0m02.19s  || -0m00.25s  | -11.41%
0m01.60s  | curve25519_64.c                                                      | 0m01.53s  || +0m00.07s  | +4.57%
0m01.41s  | Experiments/NewPipeline/CLI.vo                                       | 0m01.49s  || -0m00.08s  | -5.36%
0m01.30s  | Experiments/NewPipeline/StandaloneOCamlMain.vo                       | 0m01.25s  || +0m00.05s  | +4.00%
0m01.26s  | Experiments/NewPipeline/StandaloneHaskellMain.vo                     | 0m01.17s  || +0m00.09s  | +7.69%
0m01.04s  | Experiments/NewPipeline/CompilersTestCases.vo                        | 0m00.96s  || +0m00.08s  | +8.33%
0m00.62s  | Experiments/NewPipeline/MiscCompilerPasses.vo                        | 0m00.68s  || -0m00.06s  | -8.82%

src/Experiments/NewPipeline/MiscCompilerPasses.v
@@ -11,65 +11,6 @@ Module Compilers.
   Import invert_expr.
   Import defaults.
 
-  Module DeadCodeElimination.
-    Section with_ident.
-      Context {base_type : Type}.
-      Local Notation type := (type.type base_type).
-      Context {ident : type -> Type}.
-      Local Notation expr := (@expr.expr base_type ident).
-      Fixpoint compute_live' {t} (e : @expr (fun _ => PositiveSet.t) t) (cur_idx : positive)
-        : positive * PositiveSet.t
-        := match e with
-           | expr.Var t v => (cur_idx, v)
-           | expr.App s d f x
-             => let '(idx, live1) := @compute_live' _ f cur_idx in
-                let '(idx, live2) := @compute_live' _ x idx in
-                (idx, PositiveSet.union live1 live2)
-           | expr.Abs s d f
-             => let '(_, live) := @compute_live' _ (f PositiveSet.empty) cur_idx in
-                (cur_idx, live)
-           | expr.LetIn tx tC ex eC
-             => let '(idx, live) := @compute_live' tx ex cur_idx in
-                let '(_, live) := @compute_live' tC (eC (PositiveSet.add idx live)) (Pos.succ idx) in
-                (Pos.succ idx, live)
-           | expr.Ident t idc => (cur_idx, PositiveSet.empty)
-           end.
-      Definition compute_live {t} e : PositiveSet.t := snd (@compute_live' t e 1).
-      Definition ComputeLive {t} (e : expr.Expr t) := compute_live (e _).
-
-      Section with_var.
-        Context {var : type -> Type}
-                (live : PositiveSet.t).
-        Definition OUGHT_TO_BE_UNUSED {T1 T2} (v : T1) (v' : T2) := v.
-        Global Opaque OUGHT_TO_BE_UNUSED.
-        Fixpoint eliminate_dead' {t} (e : @expr (@expr var) t) (cur_idx : positive)
-          : positive * @expr var t
-          := match e with
-             | expr.Var t v => (cur_idx, v)
-             | expr.Ident t idc => (cur_idx, expr.Ident idc)
-             | expr.App s d f x
-               => let '(idx, f') := @eliminate_dead' _ f cur_idx in
-                  let '(idx, x') := @eliminate_dead' _ x idx in
-                  (idx, expr.App f' x')
-             | expr.Abs s d f
-               => (cur_idx, expr.Abs (fun v => snd (@eliminate_dead' _ (f (expr.Var v)) cur_idx)))
-             | expr.LetIn tx tC ex eC
-               => let '(idx, ex') := @eliminate_dead' tx ex cur_idx in
-                  let eC' := fun v => snd (@eliminate_dead' _ (eC v) (Pos.succ idx)) in
-                  if PositiveSet.mem idx live
-                  then (Pos.succ idx, expr.LetIn ex' (fun v => eC' (expr.Var v)))
-                  else (Pos.succ idx, eC' (OUGHT_TO_BE_UNUSED ex' (Pos.succ idx, PositiveSet.elements live)))
-             end.
-
-        Definition eliminate_dead {t} e : expr t
-          := snd (@eliminate_dead' t e 1).
-      End with_var.
-
-      Definition EliminateDead {t} (e : expr.Expr t) : expr.Expr t
-        := fun var => eliminate_dead (ComputeLive e) (e _).
-    End with_ident.
-  End DeadCodeElimination.
-
   Module Subst01.
     Local Notation PositiveMap_incr idx m
       := (PositiveMap.add idx (match PositiveMap.find idx m with
@@ -86,6 +27,11 @@ Module Compilers.
                   => Some n
                 | None, None => None
                 end) m1 m2).
+    Local Notation PositiveMap_contains_nz idx m
+      := match PositiveMap.find idx m with
+         | Some v => (0 <? v)%nat
+         | None => false
+         end.
     Section with_ident.
       Context {base_type : Type}.
       Local Notation type := (type.type base_type).
@@ -105,43 +51,64 @@ Module Compilers.
                 (cur_idx, live)
            | expr.LetIn tx tC ex eC
              => let '(idx, live1) := @compute_live_counts' tx ex cur_idx in
-                let '(idx, live2) := @compute_live_counts' tC (eC idx) (Pos.succ idx) in
-                (idx, PositiveMap_union live1 live2)
+                let '(idx', live2) := @compute_live_counts' tC (eC idx) (Pos.succ idx) in
+                (idx', if PositiveMap_contains_nz idx live2
+                       then PositiveMap_union live1 live2
+                       else live2)
            end.
       Definition compute_live_counts {t} e : PositiveMap.t _ := snd (@compute_live_counts' t e 1).
       Definition ComputeLiveCounts {t} (e : expr.Expr t) := compute_live_counts (e _).
 
       Section with_var.
-        Context {var : type -> Type}
+        Context (doing_subst : forall T1 T2, T1 -> T2 -> T1)
+                {var : type -> Type}
+                (max_count_to_subst : nat)
                 (live : PositiveMap.t nat).
-        Fixpoint subst01' {t} (e : @expr (@expr var) t) (cur_idx : positive)
+        Fixpoint subst0n' {t} (e : @expr (@expr var) t) (cur_idx : positive)
           : positive * @expr var t
           := match e with
              | expr.Var t v => (cur_idx, v)
              | expr.Ident t idc => (cur_idx, expr.Ident idc)
              | expr.App s d f x
-               => let '(idx, f') := @subst01' _ f cur_idx in
-                  let '(idx, x') := @subst01' _ x idx in
+               => let '(idx, f') := @subst0n' _ f cur_idx in
+                  let '(idx, x') := @subst0n' _ x idx in
                   (idx, expr.App f' x')
              | expr.Abs s d f
-               => (cur_idx, expr.Abs (fun v => snd (@subst01' _ (f (expr.Var v)) (Pos.succ cur_idx))))
+               => (cur_idx, expr.Abs (fun v => snd (@subst0n' _ (f (expr.Var v)) (Pos.succ cur_idx))))
              | expr.LetIn tx tC ex eC
-               => let '(idx, ex') := @subst01' tx ex cur_idx in
-                  let eC' := fun v => snd (@subst01' tC (eC v) (Pos.succ idx)) in
+               => let '(idx, ex') := @subst0n' tx ex cur_idx in
+                  let eC' := fun v => snd (@subst0n' tC (eC v) (Pos.succ idx)) in
                   if match PositiveMap.find idx live with
-                     | Some n => (n <=? 1)%nat
+                     | Some n => (n <=? max_count_to_subst)%nat
                      | None => true
                      end
-                  then (Pos.succ idx, eC' ex')
+                  then (Pos.succ idx, eC' (doing_subst _ _ ex' (Pos.succ idx, PositiveMap.elements live)))
                   else (Pos.succ idx, expr.LetIn ex' (fun v => eC' (expr.Var v)))
              end.
 
-        Definition subst01 {t} e : expr t
-          := snd (@subst01' t e 1).
+        Definition subst0n {t} e : expr t
+          := snd (@subst0n' t e 1).
       End with_var.
 
-      Definition Subst01 {t} (e : expr.Expr t) : expr.Expr t
-        := fun var => subst01 (ComputeLiveCounts e) (e _).
+      Definition Subst0n (doing_subst : forall T1 T2, T1 -> T2 -> T1) (max_count_to_subst : nat) {t} (e : expr.Expr t) : expr.Expr t
+        := fun var => subst0n doing_subst max_count_to_subst (ComputeLiveCounts e) (e _).
+
+      Definition Subst01 {t} (e : expr.Expr t) : expr.Expr t := Subst0n (fun _ _ x _ => x) 1 e.
     End with_ident.
   End Subst01.
+
+  Module DeadCodeElimination.
+    Section with_ident.
+      Context {base_type : Type}.
+      Local Notation type := (type.type base_type).
+      Context {ident : type -> Type}.
+      Local Notation expr := (@expr.expr base_type ident).
+
+      Definition OUGHT_TO_BE_UNUSED {T1 T2} (v : T1) (v' : T2) := v.
+      Global Opaque OUGHT_TO_BE_UNUSED.
+
+      Definition EliminateDead {t} (e : expr.Expr t) : expr.Expr t
+        := @Subst01.Subst0n base_type ident (@OUGHT_TO_BE_UNUSED) 0 t e.
+    End with_ident.
+  End DeadCodeElimination.
 End Compilers.
